src/SemanticsNew.v
@@ -1,4 +1,4 @@
-Require Import Lib.FMap Lib.Struct.
+Require Import Lib.CommonTactics Lib.FMap Lib.Struct.
 Require Import Syntax Semantics Refinement.
 Require Import String List.
 
@@ -24,13 +24,11 @@ Definition mapLabelTP {A B : Type} (f : A -> B) (l : LabelTP A)
 Definition NotBothRule (rm1 rm2 : option string) : Prop :=
   rm1 = None \/ rm2 = None.
 
-Inductive CanCombine : (RegsT * RuleLabelT) -> (RegsT * RuleLabelT) -> Prop :=
-  MkCanCombine :
-    forall u1 rm1 ds1 cs1 u2 rm2 ds2 cs2,
-      MF.Disj u1 u2 -> MF.Disj ds1 ds2 -> MF.Disj cs1 cs2 
-      -> NotBothRule rm1 rm2
-      -> CanCombine (u1, Build_LabelTP rm1 ds1 cs1) 
-                    (u2, Build_LabelTP rm2 ds2 cs2).
+Definition CanCombine (ul1 ul2: RegsT * RuleLabelT) : Prop :=
+  MF.Disj (fst ul1) (fst ul2) /\
+  NotBothRule (ruleMeth (snd ul1)) (ruleMeth (snd ul2)) /\
+  MF.Disj (dms (snd ul1)) (dms (snd ul2)) /\
+  MF.Disj (cms (snd ul1)) (cms (snd ul2)).
 
 Definition mergeLabel {A : Type} (l1 l2 : LabelTP A) : LabelTP A := 
   match l1, l2 with
@@ -249,53 +247,81 @@ Section Decomposition.
   destruct ruleMeth0; simpl; unfold id; reflexivity.
   Qed.
 
-  Lemma canCombineLeft : forall {t u1 u2 l1 l2},
-    CanCombine t (MF.union u1 u2, mergeLabel l1 l2)
-  -> CanCombine t (u1, l1).
+  Lemma canCombineLeft :
+    forall {t u1 u2 l1 l2},
+      CanCombine t (MF.union u1 u2, mergeLabel l1 l2) ->
+      CanCombine t (u1, l1).
   Proof. 
     intros.
     destruct l1 as [rm1 ds1 cs1].
     destruct l2 as [rm2 ds2 cs2].
-    inversion H; clear H; subst. 
+    unfold CanCombine in H; dest; simpl in *.
     constructor; try (eapply MF.Disj_union_1; eassumption).
-    unfold NotBothRule in *. destruct rm1; intuition.
+    unfold NotBothRule in *.
+    destruct rm1.
+    - simpl; destruct H0; [|discriminate].
+      repeat split.
+      + left; auto.
+      + eapply MF.Disj_union_1; eauto.
+      + eapply MF.Disj_union_1; eauto.
+    - repeat split.
+      + right; auto.
+      + eapply MF.Disj_union_1; eauto.
+      + eapply MF.Disj_union_1; eauto.
   Qed.
 
-  Lemma canCombineRight : forall {t u1 u2 l1 l2},
-    CanCombine t (MF.union u1 u2, mergeLabel l1 l2)
-  -> CanCombine t (u2, l2).
+  Lemma canCombineRight :
+    forall {t u1 u2 l1 l2},
+      CanCombine t (MF.union u1 u2, mergeLabel l1 l2) ->
+      CanCombine t (u2, l2).
   Proof.
     intros.
     destruct l1 as [rm1 ds1 cs1].
     destruct l2 as [rm2 ds2 cs2].
-    inversion H; clear H; subst. 
+    unfold CanCombine in H; dest; simpl in *.
     constructor; try (eapply MF.Disj_union_2; eassumption).
-    unfold NotBothRule in *. destruct rm1; intuition.
-    congruence.
+    unfold NotBothRule in *.
+    destruct rm1.
+    - simpl; destruct H0; [|discriminate].
+      repeat split.
+      + left; auto.
+      + eapply MF.Disj_union_2; eauto.
+      + eapply MF.Disj_union_2; eauto.
+    - simpl; destruct H0.
+      + repeat split.
+        * left; auto.
+        * eapply MF.Disj_union_2; eauto.
+        * eapply MF.Disj_union_2; eauto.
+      + repeat split.
+        * right; auto.
+        * eapply MF.Disj_union_2; eauto.
+        * eapply MF.Disj_union_2; eauto.
   Qed.
 
   Lemma canCombineMerge : forall {t u1 u2 l1 l2},
     CanCombine t (u1, l1)
   -> CanCombine t (u2, l2)
   -> CanCombine t (MF.union u1 u2, mergeLabel l1 l2).
-  Proof. 
-    intros. destruct t as [uL [rmL csL dsL]]. 
-    destruct (mergeLabel l1 l2) as [rm1 cs ds] eqn:labeleqn.
-    inversion H; inversion H0; inversion labeleqn; subst.
-    econstructor. apply MF.Disj_union; assumption.
-    apply MF.Disj_union; assumption.
-    apply MF.Disj_union; assumption.
-    unfold NotBothRule in *; destruct rmL, rm2, rm4; intuition.
+  Proof.
+    admit.
+    (* intros. destruct t as [uL [rmL csL dsL]].  *)
+    (* destruct (mergeLabel l1 l2) as [rm1 cs ds] eqn:labeleqn. *)
+    (* inversion H; inversion H0; inversion labeleqn; subst. *)
+    (* econstructor. apply MF.Disj_union; assumption. *)
+    (* apply MF.Disj_union; assumption. *)
+    (* apply MF.Disj_union; assumption. *)
+    (* unfold NotBothRule in *; destruct rmL, rm2, rm4; intuition. *)
   Qed.  
 
   Lemma canCombineSym : forall {t1 t2},
     CanCombine t1 t2 -> CanCombine t2 t1.
-  Proof. 
-   intros t1 t2 H;
-   inversion H; clear H; subst; 
-   constructor; eauto using MF.Disj_comm.
-   unfold NotBothRule in *.
-   destruct rm1, rm2; intuition.
+  Proof.
+    admit.
+   (* intros t1 t2 H; *)
+   (* inversion H; clear H; subst;  *)
+   (* constructor; eauto using MF.Disj_comm. *)
+   (* unfold NotBothRule in *. *)
+   (* destruct rm1, rm2; intuition. *)
   Qed. 
 
   Lemma specShouldCombines : forall {oImp} 
@@ -335,25 +361,26 @@ Require CommonTactics.
          /\ equivalent lSpec lImp pRL)
         * UnitSteps spec oSpec nSpec lSpec.
   Proof.
-    intros.
-    induction steps; intros.
-    - pose proof (consistentSubstepMap H u0). simpl in *.
-      destruct (T u0) as [uSpec lSpec].
-      intuition. constructor. assumption.
-  - pose proof (specShouldCombines H steps1 steps2 c).
-    simpl in *.
-    destruct (Ts steps1) as [uSpec1 lSpec1].
-    destruct (Ts steps2) as [uSpec2 lSpec2].
-    intuition. 
-    CommonTactics.inv c. CommonTactics.inv H0.
-    apply stateMapModular; assumption.
-    unfold equivalent in *. subst.
-    CommonTactics.inv c.
-    apply pmerge; assumption.
-    apply UnitStepsUnion. assumption. assumption.
-    unfold equivalent in *.
-    assumption.
-    Qed.
+    admit.
+  (*   intros. *)
+  (*   induction steps; intros. *)
+  (*   - pose proof (consistentSubstepMap H u0). simpl in *. *)
+  (*     destruct (T u0) as [uSpec lSpec]. *)
+  (*     intuition. constructor. assumption. *)
+  (* - pose proof (specShouldCombines H steps1 steps2 c). *)
+  (*   simpl in *. *)
+  (*   destruct (Ts steps1) as [uSpec1 lSpec1]. *)
+  (*   destruct (Ts steps2) as [uSpec2 lSpec2]. *)
+  (*   intuition.  *)
+  (*   CommonTactics.inv c. CommonTactics.inv H0. *)
+  (*   apply stateMapModular; assumption. *)
+  (*   unfold equivalent in *. subst. *)
+  (*   CommonTactics.inv c. *)
+  (*   apply pmerge; assumption. *)
+  (*   apply UnitStepsUnion. assumption. assumption. *)
+  (*   unfold equivalent in *. *)
+  (*   assumption. *)
+  Qed.
   
   Lemma consistentStepMap : forall oImp lImp nImp
     , (exists ruleLabel, Behavior imp oImp ruleLabel)
